Improved typing and fixed a proof
Don't rely on a fudge for correctness

il1Script.sml
@@ -27,15 +27,39 @@ val il1_expr_type_def = Define `
 (il1_expr_type (IL1_Value (IL1_Boolean _)) g = SOME boolL1) /\
 (il1_expr_type (IL1_Plus e1 e2) g = if (il1_expr_type e1 g = SOME intL1) /\ (il1_expr_type e2 g = SOME intL1) then SOME intL1 else NONE) /\
 (il1_expr_type (IL1_Geq e1 e2) g = if (il1_expr_type e1 g = SOME intL1) /\ (il1_expr_type e2 g = SOME intL1) then SOME boolL1 else NONE) /\
-(il1_expr_type (IL1_Deref l) g = if l ∈ FDOM g \/ (?l'.l = Compiler l') then SOME intL1 else NONE) /\
+(il1_expr_type (IL1_Deref l) g = if l ∈ g then SOME intL1 else NONE) /\
 (il1_expr_type (IL1_EIf e1 e2 e3) g = if (il1_expr_type e1 g = SOME boolL1) /\ (il1_expr_type e2 g = il1_expr_type e3 g) then (il1_expr_type e2 g) else NONE)`;
 
-val il1_type_def = Define `
-(il1_type (IL1_Expr e) g = il1_expr_type e g) /\
-(il1_type (IL1_Assign l e) g = if (l ∈ FDOM g \/ (?l'.l = Compiler l')) /\ (il1_expr_type e g = SOME intL1) then SOME unitL1 else NONE) /\
-(il1_type (IL1_Seq e1 e2) g = if (il1_type e1 g = SOME unitL1) then il1_type e2 g else NONE) /\
-(il1_type (IL1_SIf e1 e2 e3) g = if (il1_expr_type e1 g = SOME boolL1) /\ (il1_type e2 g = il1_type e3 g) then il1_type e2 g else NONE) /\
-(il1_type (IL1_While e1 e2) g = if (il1_expr_type e1 g = SOME boolL1) /\ (il1_type e2 g = SOME unitL1) then SOME unitL1 else NONE)`;
+val il1_type_pair_def = Define `
+(il1_type_pair (IL1_Expr e) g =
+    let t = il1_expr_type e g in
+    case t of SOME r => SOME (r, g) 
+           | NONE => NONE) /\
+(il1_type_pair (IL1_Assign l e) g =
+    let te = il1_expr_type e g in
+    case te of SOME intl1 => SOME (unitL1, l INSERT g) 
+	   | _ => NONE) /\
+(il1_type_pair (IL1_Seq e1 e2) g =
+    let pair = il1_type_pair e1 g in
+    case pair of SOME (unitL1, g') => il1_type_pair e2 g' 
+	   | _ => NONE) /\
+(il1_type_pair (IL1_SIf e1 e2 e3) g =
+    let t = il1_expr_type e1 g in
+        case t of SOME boolL1 =>
+                  (let pair1 = il1_type_pair e2 g in
+                       case pair1 of SOME (t, g') =>
+                           (let pair2 = il1_type_pair e3 g' in
+                               case pair2 of SOME (t, g'') => SOME (t, g' ∪ g'') 
+					  | _ => NONE)
+				  | _ => NONE)
+	       | _ => NONE) /\
+(il1_type_pair (IL1_While e1 e2) g =
+    let t = il1_expr_type e1 g in
+        case t of SOME boolL1 =>
+            (let pair = il1_type_pair e2 g in
+                 case pair of SOME (unitL1, g') => SOME (unitL1, g') 
+			   | _ => NONE)
+	       | _ => NONE)`;
 
 val contains_expr_def = Define `
     (contains_expr l (IL1_Value v) = F) /\
@@ -121,6 +145,20 @@ THEN1 (imp_res_tac BS_IL1_EXPR_GEQ_BACK_THM THEN res_tac THEN rw [])
 THEN1 (imp_res_tac BS_IL1_EXPR_DEREF_BACK_THM THEN rw [])
 THEN1 (imp_res_tac BS_IL1_EXPR_EIF_BACK_THM THEN res_tac THEN rw [])
 THEN1 (imp_res_tac BS_IL1_EXPR_EIF_BACK_THM THEN res_tac THEN rw []));
+
+val BS_IL1_EXPR_TYPE_INT = store_thm("BS_IL1_EXPR_TYPE_INT",
+``!e s.((il1_expr_type e s = SOME intL1) ==> ?n.bs_il1_expr (e, s) (IL1_Integer n)) /\ ((il1_expr_type e s = SOME boolL1) ==> ?bo.bs_il1_expr (e, s) (IL1_Boolean bo)) /\ ((il1_expr_type e s = SOME unitL1) ==> bs_il1_expr (e, s) IL1_ESkip)``,
+Induct_on `e` THEN1 (Cases_on `i` THEN fs [il1_expr_type_def, Once bs_il1_expr_cases, FDOM_DEF] THEN fs [il1_expr_type_def] THEN EVAL_TAC THEN rw [Once bs_il1_expr_cases])
+
+THEN EVAL_TAC
+THEN fs [il1_expr_type_def]
+THEN rw []
+THEN imp_res_tac EQ_SYM
+THEN imp_res_tac EQ_TRANS
+THEN res_tac
+THEN rw [Once bs_il1_expr_cases]
+THEN (TRY (metis_tac []))
+THENL [Cases_on `bo`, Cases_on `bo''`, Cases_on `bo`] THEN metis_tac []);
 
 val (bs_il1_rules, bs_il1_induction, bs_il1_cases) = Hol_reln `
     (*  Expressions *)
